add httpProtocolMock

httpProtocolMock/funcHelpers.c
@@ -1,15 +1,15 @@
 #include <stdio.h>
 #include <stdlib.h>
+#include <string.h>
 #include <inttypes.h>
 
-#include "Server.h"
+#include "HttpProtocolMock.h"
 
 char char_of_uint8(uint8_t x) {
   return (char) x;
 }
 
 uint32_t bufstrcpy(char *dst, const char *src) {
-  /* The F* precondition guarantees that src is zero-terminated */
   return sprintf(dst, "%s", src);
 }
 
