httpProtocolMock/httpCliantMock.c
@@ -1,0 +1,50 @@
+#include <stdio.h>
+#include <stdlib.h>
+
+#include "HttpProtocolMock.h"
+
+int main(int argc, char *argv[]) {
+  if (argc != 2) {
+    puts("./a.out '(GET|POST) REQUEST'");
+    return 1;
+  }
+
+  char response[2048];
+  const char *request = argv[1];
+  uint32_t n = server((char *) request, response);
+
+  FILE *fp;
+
+  fp = fopen("/tmp/response.txt", "w");
+  if (fp == NULL) {
+    puts("cannot open file.");
+    return 1;
+  }
+
+  fprintf(fp, "%s", response);
+
+  uint32_t r_count = 0;
+  uint32_t n_count = 0;
+
+  for (int i = 0; i < strlen(response); i++)
+  {
+    if (response[i] == '\r') {
+      r_count++;
+    } else if (response[i] == '\n') {
+      n_count++;
+    } else {
+      if (r_count == 2 && n_count == 2) {
+        for (int j = i; j < strlen(response); j++) {
+          printf("%c", response[j]);
+        }
+        puts("");
+        return 0;
+      } else {
+        r_count = 0;
+        n_count = 0;
+      }
+    }
+  }
+  puts("request may be invalid.");
+  return 1;
+}
