Makefile
@@ -19,5 +19,3 @@ forUint32:
 
 fizzBuzz:
 	krml -verify -drop WasmSupport -tmpdir ./out -no-prefix FizzBuzz fizzBuzz.fst && ./a.out
-server:
-	krml -verify -drop WasmSupport -tmpdir ./out -no-prefix Server Server.fst main-Server.c helpers-Server.c && ./a.out
