httpProtocolMock/httpProtocolMock.sh
@@ -1,0 +1,36 @@
+requestType=$1
+url=$2
+argc=$#
+howToUse='ex: ./httpProtocolMock.sh "GET" "/"'
+exexFile="./a.out"
+
+if [ $argc != 2 ]; then
+    echo $howToUse
+    exit 1
+fi
+
+if [ ! -e $exexFile ]; then
+    echo "Please generate exec-file before running this script."
+    exit 1
+fi
+
+./a.out $requestType" "$url" HTTP/1.1\r\n" > /tmp/index.html;
+ret=$?
+if [ $ret = 0 ]; then
+    echo [response]
+    echo "------------------------------------------------"
+    cat "/tmp/response.txt"
+    echo -e "\n------------------------------------------------\n"
+    echo [parsed response]
+    echo "------------------------------------------------"
+    cat /tmp/index.html
+    echo "------------------------------------------------"
+    echo "Open browser..."
+    open "/tmp/index.html"
+    echo "Done!"
+    exit 0
+else
+    cat /tmp/index.html
+    echo $howToUse
+    exit 1
+fi
